examples/sbf/FilterRepr.v
@@ -14,7 +14,7 @@ Section FilterRepr.
 Notation ident := string.
 Notation path := (list ident).
 
-Context {num_rows num_slots : Z}.
+Context {num_frames num_rows num_slots : Z}.
 
 Definition bool_to_val (b : bool) : ValueBase :=
   ValBaseBit [b; false; false; false; false; false; false; false].
@@ -67,5 +67,31 @@ Definition timer_repr_val (t : Z * bool) :=
 Definition timer_repr (p : path) (t : Z * bool) : ext_pred :=
   (ExtPred.singleton (p ++ ["reg_clear_window"])
         (Tofino.ObjRegister [timer_repr_val t])).
+
+Program Definition filter_repr (p : path) (w : N) (panes : list string) (rows : list string) (cf : ConFilter.filter num_frames num_rows num_slots) : ext_pred :=
+  let 'mk_filter pns clear_index timer := cf in
+  ExtPred.wrap [p] (
+    map2 (fun pane cpa => frame_repr (p ++ [pane]) rows cpa) panes pns ++
+    [fil_clear_index_repr p w clear_index] ++
+    [timer_repr p timer]) _.
+Next Obligation.
+  rewrite forallb_app, Reflect.andE; split.
+  2 : simpl; rewrite Reflect.andE; split.
+  - unfold map2. generalize (combine panes (proj1_sig pns)) as panes_pns.
+    clear; intros.
+    induction panes_pns; auto.
+    destruct a.
+    simpl.
+    rewrite IHpanes_pns.
+    unfold in_scope.
+    rewrite <- (app_nil_r p) at 1.
+    rewrite is_prefix_cancel. auto.
+  - unfold in_scope.
+    rewrite <- (app_nil_r p) at 1.
+    rewrite is_prefix_cancel. auto.
+  - unfold in_scope.
+    rewrite <- (app_nil_r p) at 1.
+    rewrite is_prefix_cancel. auto.
+Qed.
 
 End FilterRepr.
